

## Tutorial - 2

$$Q.1) \quad T(n) = \begin{cases} 7T\left(\frac{n}{2}\right) + n^2 & \text{if } n > 2 \\ 1 & \text{if } n \leq 2 \end{cases}$$

$$\rightarrow T(n) = 7T\left(\frac{n}{2}\right) + n^2$$

$$= 7\left[7T\left(\frac{n}{2^2}\right) + \left(\frac{n}{2}\right)^2\right] + n^2$$

$$= 7^2 T\left(\frac{n}{2^2}\right) + 7\left(\frac{n}{2}\right)^2 + n^2$$

$$= 7^2 \left[7T\left(\frac{n}{2^3}\right) + \left(\frac{n}{2^2}\right)^2\right] + 7\left(\frac{n}{2}\right)^2 + n^2$$

$$= 7^3 T\left(\frac{n}{2^3}\right) + 7^2 \left(\frac{n}{2^2}\right)^2 + 7\left(\frac{n}{2}\right)^2 + n^2$$

⋮

$$= 7^k T\left(\frac{n}{2^k}\right) + 7^{k-1} \left(\frac{n}{2^{k-1}}\right)^2 + \dots + 7^2 \left(\frac{n}{2^2}\right)^2 + 7\left(\frac{n}{2}\right)^2 + n^2$$

$$= 7^k T\left(\frac{n}{2^k}\right) + \sum_{i=1}^{k-1} 7^i \left(\frac{n}{2^i}\right)^2 + n^2$$

$$\text{as } \frac{n}{2^k} = 1 \quad \therefore n = 2^k$$

$$\therefore k = \log_2 n$$

$$\therefore = 7^{\log_2 n} (1) + \sum_{i=1}^{\log_2 n - 1} 7^i \left(\frac{n}{2^i}\right)^2 + n^2$$

$$= 7^{\log_2 n} + n^2$$

$$= n^{\log_2 7} + n^2$$

$$\Rightarrow O(n^{\log_2 7})$$

Q.2)  $T(n) = \begin{cases} T(1) & \text{if } n=0 \\ 2T\left(\frac{n}{2}\right) + n & \text{if } n \neq 1 \end{cases}$

$$\rightarrow T(n) = 2T\left(\frac{n}{2}\right) + n$$

$$= 2 \left[ 2T\left(\frac{n}{2^2}\right) + \frac{n}{2} \right] + n$$

$$= 2^2 T\left(\frac{n}{2^2}\right) + \frac{2n}{2} + n$$

$$= 2^2 T\left(\frac{n}{2^2}\right) + 2n$$

$$= 2^2 \left[ 2T\left(\frac{n}{2^3}\right) + \frac{n}{2^2} \right] + 2n$$

$$= 2^3 T\left(\frac{n}{2^3}\right) + \frac{2^2 \cdot n}{2^2} + 2n$$

$$= 2^3 T\left(\frac{n}{2^3}\right) + 3n$$

⋮

$$= 2^k T\left(\frac{n}{2^k}\right) + k \cdot n$$

as  $\frac{2^k}{n} = 1 \therefore 2^k = n$   
 $\therefore k = \log_2 n$

$$= n \cdot (1) + \log_2 n \times n$$

$$= n \log n + n$$

$$\boxed{T(n) = O(n \log n)}$$

$$Q.3) \quad T(n) = \begin{cases} 9 & n=0 \\ 2T(n/2) + bn & n>1 \end{cases}$$

$$\longrightarrow T(n) = 2T\left(\frac{n}{2}\right) + bn$$

$$= 2 \left[ 2T\left(\frac{n}{2^2}\right) + b\left(\frac{n}{2}\right) \right] + bn$$

$$= 2^2 T\left(\frac{n}{2^2}\right) + bn + bn$$

$$= 2^2 T\left(\frac{n}{2}\right) + 2bn$$

$$= 2^2 \left[ 2T\left(\frac{n}{2^3}\right) + b \frac{n}{2^2} \right] + 2bn$$

$$= 2^3 T\left(\frac{n}{2^3}\right) + bn + 2bn$$

$$= 2^3 T\left(\frac{n}{2^3}\right) + 3bn$$

|  
|  
|

$$= 2^k T\left(\frac{n}{2^k}\right) + k \cdot bn$$

$$\text{as } 2^k = n \\ k = \log_2 n$$

$$\therefore = 2 \cdot n \cdot (1) + \log_2 n \cdot bn$$

$$\therefore T(n) = O(n \log_2 n)$$

$$\text{Q.4)} \quad T(n) = \begin{cases} C & n=1 \\ 2T(n/2) + C & n>1 \end{cases}$$

$$\rightarrow T(n) = 2T\left(\frac{n}{2}\right) + C$$

$$= 2 \left[ 2T\left(\frac{n}{2^2}\right) + C \right] + C$$

$$= 2^2 T\left(\frac{n}{2^2}\right) + 2C + C$$

$$= 2^2 \left[ 2T\left(\frac{n}{2^3}\right) + C \right] + 2C + C$$

$$= 2^3 T\left(\frac{n}{2^3}\right) + 2^2 C + 2^1 C + 2^0 C$$

⋮

$$= 2^k T\left(\frac{n}{2^k}\right) + 2^{k-1} C + \dots + 2^2 C + 2^1 C + 2^0 C$$

$$= 2^k T\left(\frac{n}{2^k}\right) + (2^k - 1)C$$

$$\text{as } 2^k = n$$

$$k = \log_2 n$$

$$= n \cdot (1) + (2^{\log_2 n} - 1)C$$

$$= O(n)$$

$$\boxed{T(n) = O(n)}$$

Q.5) recursive algorithm of factorial and its recurrence relation.

→

fact(n)  $\rightarrow T(n)$   
{  
  if  $n=0$  ||  $n=1$  then  $\rightarrow 1$   
    return 1;  
  else  
    return fact(n-1) \* n;  $\rightarrow T(n-1)$   
}

$$T(n) = T(n-1) + 1$$

$$\therefore T(n) = T(n-1) + 1$$

$$= T(n-1-1) + 1 + 1$$

$$= T(n-2) + 2$$

$$= T(n-2-1) + 1 + 2$$

$$= T(n-3) + 3$$

⋮

$$= T(n-k) + k.$$

$$n-k=0$$

$$n=k$$

$$\therefore T(n) = T(0) + n$$

$$T(n) = n$$

$$\boxed{T(n) = O(n)}$$

Q.6) recursive algorithm of fibonacci series and solve recurrence relation.

```

fibonacci(n)           T(n)
{
    if n <= 1           — 1
        return n;
    else
        return fibonacci(n-1) + fibonacci(n-2); — T(n-1) + T(n-2)
}

```

$$\therefore T(n) = T(n-1) + T(n-2) + c$$

$$\text{Assume } T(n-1) \approx T(n-2)$$

$$\begin{aligned}
 \therefore T(n) &= 2T(n-2) + c \\
 &= 2[2T(n-4) + c] + c \\
 &= 4T(n-4) + 2c + c \\
 &= 4[2T(n-6) + c] + 2c + c \\
 &= 8T(n-6) + 4c + 2c + c \\
 &= 2^3 T(n-6) + 2^2 c + 2^1 c + 2^0 c \\
 &\vdots
 \end{aligned}$$

$$= 2^k T(n-2k) + (2^k - 1)c$$

$$\begin{aligned}
 \therefore n-2k &= 0 \quad \therefore n = 2k \\
 k &= n/2
 \end{aligned}$$

$$T(n) = 2^{n/2} T(0) + (2^{n/2} - 1)c$$

$$T(n) \propto 2^{n/2} \text{ (lower bound)}$$

now assume,

$$T(n-2) \approx T(n-1)$$

$$\begin{aligned}\therefore T(n) &= 2T(n-1) + C \\ &= 2[2T(n-2) + C] + C\end{aligned}$$

$$= 2^2 T(n-2) + 2C + C$$

$$= 2^2 [2T(n-3) + C] + 2C + C$$

$$= 2^3 T(n-3) + 2^2 C + 2^1 C + 2^0 C$$

!

:

$$= 2^k T(n-k) + (2^k - 1)C$$

$$\therefore n-k=0 \quad \therefore k=n$$

$$= 2^n \cdot T(0) + (2^n - 1)C$$

$$T(n) \propto 2^n \text{ (upper bound)}$$

$$\therefore \boxed{T(n) = O(2^n)}$$

Q.7) Show that the following equalities are correct

a)  $5n^2 - 6n \Rightarrow O(n^2)$

$$f(n) = 5n^2 - 6n$$

for time complexity we take term with highest degree and neglect coefficient.  
so,

$$\underline{O(n^2)}$$

b)  ~~$n! \Rightarrow O(n^n)$~~

b)  $n^3 + 10^6 n^2 \Rightarrow O(n^3)$

$$f(n) = n^3 + 10^6(n^2)$$

here we take highest degree term of  $n$  i.e.  $n^3$

so,

$$\underline{O(n^3)}$$

Q.8) show that the following equalities are incorrect.

a)  $10n^2 + 9 \Rightarrow O(n)$   
 $f(n) = 10n^2 + 9$

here for time complexity we select highest degree term of  $n$  and coefficient of that term neglected so,

$$\Rightarrow O(n^2)$$

so  $O(n)$  is incorrect.

b)  $n^2 \log n \Rightarrow O(n^2)$   
 $f(n) = n^2 \log n$

as here only one term of  $n$  so  $O(n^2 \log n)$  so  $O(n^2)$  is incorrect.

c)  $\frac{n^2}{\log n} \Rightarrow O(n^2)$

$$f(n) = \frac{n^2}{\log n}$$

as here only one term of  $n$  so  $O(n^2 / \log n)$  so  $O(n^2)$  is incorrect.